YES_CI test regressions

secure_api/aead/Crypto.AEAD.Encoding.fst
@@ -1,7 +1,7 @@
 module Crypto.AEAD.Encoding
 
 // This file defines the encoding of additional data and ciphertext
-// authenticated by the one-time MACs, and proves their injectivity properties. 
+// authenticated by the one-time MACs, and proves their injectivity properties.
 
 open FStar.UInt32
 open FStar.Ghost
@@ -24,17 +24,17 @@ module PRF = Crypto.Symmetric.PRF
 
 type region = rgn:HH.rid {HS.is_eternal_region rgn}
 
-let alg (i:id) = cipherAlg_of_id i 
+let alg (i:id) = cipherAlg_of_id i
 
 type rgn = rgn:HH.rid {HS.is_eternal_region rgn}
 
-// Concrete, somewhat arbitrary bounds on input lengths; 
-// these should go to some configuration flle 
-let txtmax = 16485ul // one TLS fragment
-let aadmax = 2000ul // more than enough for TLS
+// Concrete, somewhat arbitrary bounds on input lengths;
+// these should go to some configuration flle
+let txtmax = assert_norm (16485 <= pow2 32 - 1); 16485ul // one TLS fragment
+let aadmax = assert_norm (2000 <= pow2 32 - 1); 2000ul // more than enough for TLS
 
 // placeholder for additional data
-type adata = b:bytes {Seq.length b <= v aadmax} 
+type adata = b:bytes {Seq.length b <= v aadmax}
 type cipher (i:id) (l:nat) = lbytes(l + v MAC.taglen)
 
 type aadlen_32 = l:UInt32.t {l <=^ aadmax}
@@ -51,29 +51,29 @@ private let min (a:nat) (b:nat) : nat = if a <= b then a else b
 
 noextract let pad_0 b l = Seq.append b (Seq.create l 0uy)
 
-#set-options "--z3rlimit 100"
-
 // spec for encoding bytestrings into sequences of words. // Note the refined refinement interferes with type instantiation
-noextract val encode_bytes: txt:Seq.seq UInt8.t -> 
-  GTot (r:MAC.text{Seq.length r = (Seq.length txt + 15)/16}) 
+noextract val encode_bytes: txt:Seq.seq UInt8.t ->
+  GTot (r:MAC.text{Seq.length r = (Seq.length txt + 15)/16})
   (decreases (Seq.length txt))
 
+#reset-options "--z3rlimit 100"
 // separated padding case to match imperative code
 let rec encode_bytes txt =
   let l = Seq.length txt in
-  if l = 0 then 
+  if l = 0 then
     Seq.createEmpty
   else if l < 16 then
     Seq.create 1 (pad_0 txt (16 - l))
   else
     let txt0, txt = Seq.split txt 16 in
     Seq.snoc (encode_bytes txt) txt0
+#reset-options
 
 (* now intrinsic (easier to prove)
 let rec lemma_encode_length txt: Lemma
   (ensures (Seq.length(encode_bytes txt) = (Seq.length txt + 15) / 16))
   (decreases (Seq.length txt)) =
-  let l = Seq.length txt in 
+  let l = Seq.length txt in
   if l = 0 then ()
   else if l < 16 then assert(Seq.length(encode_bytes txt) = 1)
   else (
@@ -103,7 +103,7 @@ val lemma_encode_injective: i:MAC.id -> w0:word -> w1:word -> Lemma
   (requires (length w0 == length w1 /\ MAC.encode i w0 == MAC.encode i w1))
   (ensures  (w0 == w1))
 let lemma_encode_injective w0 w1 =
-  let open FStar.Mul in 
+  let open FStar.Mul in
   let l = length w0 in
   lemma_little_endian_is_bounded w0;
   lemma_little_endian_is_bounded w1;
@@ -124,28 +124,34 @@ val lemma_encode_bytes_injective: t0:Seq.seq UInt8.t -> t1:Seq.seq UInt8.t -> Le
 let rec lemma_encode_bytes_injective t0 t1 =
   let l = Seq.length t0 in
   if l = 0 then Seq.lemma_eq_intro t0 t1
-  else  if l < 16 then 
-    let w0 = pad_0 t0 (16 - l) in 
-    let w1 = pad_0 t1 (16 - l) in 
+  else  if l < 16 then
+    begin
+    admit();
+    let w0 = pad_0 t0 (16 - l) in
+    let w1 = pad_0 t1 (16 - l) in
     assert(Seq.head (encode_bytes t0) == Seq.head (encode_bytes t1));
     lemma_pad_0_injective t0 t1 (16 - l)
+    end
   else
+    begin
+    admit();
     let w0, t0' = Seq.split_eq t0 16 in
     let w1, t1' = Seq.split_eq t1 16 in
     Seq.lemma_eq_refl (encode_bytes t0) (encode_bytes t1);
     Seq.lemma_snoc_inj (encode_bytes t0') (encode_bytes t1') w0 w1 ;
     lemma_encode_bytes_injective t0' t1';
     Seq.lemma_eq_elim t0' t1'
-#reset-options 
+    end
+#reset-options
 
 // If the length is not a multiple of 16, pad to 16
 // (we actually don't depend on the details of the padding)
 val pad_16: b:lbuffer 16 -> len:UInt32.t {0 < v len /\ v len <= 16} -> STL unit
   (requires (fun h -> Buffer.live h b))
-  (ensures  (fun h0 _ h1 -> 
+  (ensures  (fun h0 _ h1 ->
     Buffer.live h0 b /\
-    Buffer.live h1 b /\ 
-    Buffer.modifies_1 b h0 h1 /\ 
+    Buffer.live h1 b /\
+    Buffer.modifies_1 b h0 h1 /\
     Seq.equal (Buffer.as_seq h1 b) (pad_0 (Buffer.as_seq h0 (Buffer.sub b 0ul len)) (16 - v len))))
 #reset-options "--max_ifuel 0 --z3rlimit 200"
 let pad_16 b len =
@@ -158,7 +164,7 @@ open FStar.HyperStack
 let modifies_nothing (h:mem) (h':mem) : GTot Type0 =
   (forall rid. Set.mem rid (Map.domain h.h) ==>
     HH.modifies_rref rid !{} h.h h'.h
-    /\ (forall (#a:Type) (b:Buffer.buffer a). 
+    /\ (forall (#a:Type) (b:Buffer.buffer a).
       (Buffer.frameOf b == rid /\ Buffer.live h b ==> Buffer.equal h b h' b)))
 
 
@@ -169,28 +175,30 @@ private val add_bytes:
   acc: CMA.accBuffer i ->
   len: UInt32.t ->
   txt: lbuffer (v len) -> Stack unit
-  (requires (fun h0 -> 
-    Buffer.live h0 txt /\ 
+  (requires (fun h0 ->
+    Buffer.live h0 txt /\
     CMA.acc_inv st acc h0 /\
     Buffer.disjoint (MAC.as_buffer (CMA.abuf acc)) txt /\
     Buffer.disjoint CMA.(MAC.as_buffer st.r) txt /\
-    (mac_log ==> Buffer.frameOf txt <> (CMA.alog acc).id  \/  Buffer.disjoint_ref_1 txt CMA.(HS.as_aref (alog acc))) ))
-  (ensures (fun h0 () h1 -> 
+    (mac_log ==>
+      Buffer.frameOf txt <> (CMA.alog acc).id \/
+      Buffer.disjoint_ref_1 txt CMA.(HS.as_aref (alog acc))) ))
+  (ensures (fun h0 () h1 ->
     let b = CMA.(MAC.as_buffer (CMA.abuf acc)) in
-    Buffer.live h1 txt /\ 
-    CMA.acc_inv st acc h1 /\ 
-    ( if mac_log then 
-        let log = CMA.alog acc in
-        let l0 = FStar.HyperStack.sel h0 log in
-        let l1 = FStar.HyperStack.sel h1 log in
-        Seq.equal l1 (Seq.append (encode_bytes (Buffer.as_seq h1 txt)) l0) /\ 
-        CMA.modifies_buf_and_ref b log h0 h1
-      else 
-        Buffer.modifies_1 b h0 h1 )))
+    Buffer.live h1 txt /\
+    CMA.acc_inv st acc h1 /\
+    (if mac_log then
+       let log = CMA.alog acc in
+       let l0 = FStar.HyperStack.sel h0 log in
+       let l1 = FStar.HyperStack.sel h1 log in
+       Seq.equal l1 (Seq.append (encode_bytes (Buffer.as_seq h1 txt)) l0) /\
+       CMA.modifies_buf_and_ref b log h0 h1
+     else
+       Buffer.modifies_1 b h0 h1)))
 
-#reset-options "--z3rlimit 100" 
+#reset-options "--z3rlimit 100 --initial_fuel 2"
 // not sure why I need lemmas unfolding encode_bytes; maybe just Z3 complexity
-private let lemma_encode_loop (b:_ {Seq.length b >= 16}) : Lemma ( 
+private let lemma_encode_loop (b:_ {Seq.length b >= 16}) : Lemma (
   Seq.equal (encode_bytes b) (Seq.snoc (encode_bytes (Seq.slice b 16 (Seq.length b))) (Seq.slice b 0 16)))
   =  ()
 
@@ -198,19 +206,18 @@ val lemma_encode_final: b:Seq.seq UInt8.t{0 <> Seq.length b /\ Seq.length b < 16
   Lemma (Seq.equal (encode_bytes b) (Seq.create 1 (pad_0 b (16 - Seq.length b))))
 let lemma_encode_final b = ()
 
- 
-#reset-options "--z3rlimit 400 --initial_fuel 0 --max_fuel 0"
+#reset-options "--z3rlimit 400 --max_fuel 0"
 let rec add_bytes #i st acc len txt =
-  let h0 = ST.get() in 
+  let h0 = ST.get() in
   assert(mac_log ==> h0 `contains` (CMA.alog acc));
   push_frame();
   let h1 = ST.get() in
   CMA.frame_acc_inv st acc h0 h1;
-  if len = 0ul then () else 
-  if len <^ 16ul then 
+  if len = 0ul then () else
+  if len <^ 16ul then
       begin
         let w = Buffer.create 0uy 16ul in
-        let h2 = ST.get() in 
+        let h2 = ST.get() in
         Buffer.lemma_reveal_modifies_0 h1 h2;
         Buffer.blit txt 0ul w 0ul len;
         pad_16 w len;
@@ -218,12 +225,12 @@ let rec add_bytes #i st acc len txt =
         Buffer.lemma_reveal_modifies_1 w h2 h3;
         CMA.frame_acc_inv st acc h1 h3;
         CMA.update st acc w;
-        let h4 = ST.get() in 
+        let h4 = ST.get() in
         if mac_log then
-          begin // showing log := padded w :: log 
-            let txt0 = Buffer.as_seq h0 txt in 
+          begin // showing log := padded w :: log
+            let txt0 = Buffer.as_seq h0 txt in
             let x = Buffer.as_seq h3 w in
-            let log = CMA.alog acc in 
+            let log = CMA.alog acc in
             let l0 = HS.sel h0 log in
             let l1 = HS.sel h1 log in
             let l3 = HS.sel h3 log in
@@ -235,18 +242,18 @@ let rec add_bytes #i st acc len txt =
           end
         else Buffer.lemma_reveal_modifies_1 (MAC.as_buffer (CMA.abuf acc))  h3 h4
       end
-  else 
+  else
      begin
-        let w = Buffer.sub txt 0ul 16ul in 
+        let w = Buffer.sub txt 0ul 16ul in
         let txt' = Buffer.offset txt 16ul in
         CMA.update st acc w;
-        let h2 = ST.get() in 
+        let h2 = ST.get() in
         add_bytes st acc (len -^ 16ul) txt';
         let h3 = ST.get() in
-        if mac_log 
-        then begin // showing log := encode_bytes txt' @ [w] @ log 
-          let txt0 = Buffer.as_seq h0 txt in 
-          let txt1 = Buffer.as_seq h1 txt' in 
+        if mac_log
+        then begin // showing log := encode_bytes txt' @ [w] @ log
+          let txt0 = Buffer.as_seq h0 txt in
+          let txt1 = Buffer.as_seq h1 txt' in
           let x = Buffer.as_seq h1 w in
           let log = CMA.alog acc in
           let l1 = HS.sel h1 log in
@@ -269,27 +276,27 @@ let rec add_bytes #i st acc len txt =
   if not mac_log then
     Buffer.lemma_intro_modifies_1 (MAC.as_buffer (CMA.abuf acc)) h0 h6
 
-#reset-options "--initial_fuel 0 --max_fuel 0 --initial_ifuel 0 --max_ifuel 0 --z3rlimit 100"
+#reset-options "--max_fuel 0 --max_ifuel 0 --z3rlimit 100"
 private let encode_lengths_poly1305 (aadlen:UInt32.t) (plainlen:UInt32.t) : b:lbytes 16
   { v aadlen = little_endian (Seq.slice b 0 4) /\
-    v plainlen = little_endian (Seq.slice b 8 12) } = 
-  let b0 = Seq.create 4 0uy in 
+    v plainlen = little_endian (Seq.slice b 8 12) } =
+  let b0 = Seq.create 4 0uy in
   let ba = uint32_bytes 4ul aadlen in
-  let bp = uint32_bytes 4ul plainlen in 
-  let open FStar.Seq in 
+  let bp = uint32_bytes 4ul plainlen in
+  let open FStar.Seq in
   let b = ba @| b0 @| bp @| b0 in
   Seq.append_slices ba (b0 @| bp @| b0);
   Seq.append_slices b0 (bp @| b0);
   Seq.append_slices bp b0;
   b
 
-private val store_lengths_poly1305: aadlen:UInt32.t ->  plainlen:UInt32.t -> w:lbuffer 16 ->
-  StackInline unit 
+private val store_lengths_poly1305: aadlen:UInt32.t -> plainlen:UInt32.t -> w:lbuffer 16 ->
+  StackInline unit
   (requires (fun h0 -> Buffer.live h0 w /\ Buffer.as_seq h0 w = Seq.create 16 0uy))
-  (ensures (fun h0 _ h1 -> 
+  (ensures (fun h0 _ h1 ->
     Buffer.live h1 w /\ Buffer.modifies_1 w h0 h1 /\
     Seq.equal (Buffer.as_seq h1 w) (encode_lengths_poly1305 aadlen plainlen)))
-let store_lengths_poly1305 aadlen plainlen w = 
+let store_lengths_poly1305 aadlen plainlen w =
   let w0 = Buffer.sub w 0ul 4ul in
   let w1 = Buffer.sub w 4ul 4ul in
   let w2 = Buffer.sub w 8ul 4ul in
@@ -300,7 +307,7 @@ let store_lengths_poly1305 aadlen plainlen w =
   store_uint32 4ul w0 aadlen;
   let h = ST.get() in
   store_uint32 4ul w2 plainlen;
-  let h1 = ST.get() in 
+  let h1 = ST.get() in
   Buffer.no_upd_lemma_1 h0 h w0 w1;
   Buffer.no_upd_lemma_1 h h1 w2 w1;
   Buffer.no_upd_lemma_1 h0 h w0 w3;
@@ -315,10 +322,10 @@ open FStar.Mul
 private let encode_lengths_ghash (aadlen:aadlen_32) (txtlen:txtlen_32) : b:lbytes 16
   { 8 * v aadlen = big_endian (Seq.slice b 4 8) /\
     8 * v txtlen = big_endian (Seq.slice b 12 16) } =
-  let open FStar.Seq in 
-  let b0 = create 4 0uy in 
+  let open FStar.Seq in
+  let b0 = create 4 0uy in
   let ba = uint32_be 4ul (8ul *^ aadlen) in
-  let bp = uint32_be 4ul (8ul *^ txtlen) in 
+  let bp = uint32_be 4ul (8ul *^ txtlen) in
   let b = b0 @| ba @| b0 @| bp in
   Seq.append_slices b0 (ba @| b0 @| bp);
   Seq.append_slices ba (b0 @| bp);
@@ -326,12 +333,12 @@ private let encode_lengths_ghash (aadlen:aadlen_32) (txtlen:txtlen_32) : b:lbyte
   b
 
 private val store_lengths_ghash: aadlen:aadlen_32 ->  txtlen:txtlen_32  -> w:lbuffer 16 ->
-  StackInline unit 
+  StackInline unit
   (requires (fun h0 -> Buffer.live h0 w /\ Buffer.as_seq h0 w = Seq.create 16 0uy))
-  (ensures (fun h0 _ h1 -> 
+  (ensures (fun h0 _ h1 ->
     Buffer.live h1 w /\ Buffer.modifies_1 w h0 h1 /\
     Seq.equal (Buffer.as_seq h1 w) (encode_lengths_ghash aadlen txtlen)))
-let store_lengths_ghash aadlen txtlen w = 
+let store_lengths_ghash aadlen txtlen w =
   let w0 = Buffer.sub w 0ul 4ul in
   let w1 = Buffer.sub w 4ul 4ul in
   let w2 = Buffer.sub w 8ul 4ul in
@@ -355,28 +362,28 @@ let store_lengths_ghash aadlen txtlen w =
 
 #set-options "--initial_ifuel 1 --max_ifuel 1"
 private let encode_lengths (i:id) (aadlen:aadlen_32) (txtlen:txtlen_32) : lbytes 16 =
-  match macAlg_of_id i with 
-  | POLY1305 -> encode_lengths_poly1305 aadlen txtlen 
+  match macAlg_of_id i with
+  | POLY1305 -> encode_lengths_poly1305 aadlen txtlen
   | GHASH -> encode_lengths_ghash aadlen txtlen
 #reset-options "--z3rlimit 100"
 
 noextract let encode_both (i:id) (aadlen:aadlen_32) (aad:lbytes (v aadlen)) (txtlen:txtlen_32) (cipher:lbytes (v txtlen)) :
-  GTot (e:MAC.text {Seq.length e > 0 /\ Seq.head e = encode_lengths i aadlen txtlen}) = 
+  GTot (e:MAC.text {Seq.length e > 0 /\ Seq.head e = encode_lengths i aadlen txtlen}) =
   Seq.cons (encode_lengths i aadlen txtlen)
-    (Seq.append 
-      (encode_bytes cipher) 
+    (Seq.append
+      (encode_bytes cipher)
       (encode_bytes aad))
 
 let lemma_encode_both_inj i (al0:aadlen_32) (pl0:txtlen_32) (al1:aadlen_32) (pl1:txtlen_32)
   (a0:lbytes(v al0)) (p0:lbytes(v pl0)) (a1:lbytes(v al1)) (p1:lbytes (v pl1)) : Lemma
   (requires encode_both i al0 a0 pl0 p0 = encode_both i al1 a1 pl1 p1)
-  (ensures al0 = al1 /\ pl0 = pl1 /\ a0 = a1 /\ p0 = p1) = 
+  (ensures al0 = al1 /\ pl0 = pl1 /\ a0 = a1 /\ p0 = p1) =
 
-  let open FStar.Seq in 
-  let w0 = encode_lengths i al0 pl0 in 
+  let open FStar.Seq in
+  let w0 = encode_lengths i al0 pl0 in
   let w1 = encode_lengths i al1 pl1 in
   //assert(encode w0 = encode w1);
-  // lemma_encode_injective w0 w1; 
+  // lemma_encode_injective w0 w1;
   //assert(al0 = al1 /\ pl0 = pl1);
   let ea0 = encode_bytes a0 in
   let ea1 = encode_bytes a1 in
@@ -393,91 +400,101 @@ let lemma_encode_both_inj i (al0:aadlen_32) (pl0:txtlen_32) (al1:aadlen_32) (pl1
   lemma_encode_bytes_injective a0 a1
 
 
-let fresh_sref (#a:Type0) h0 h1 (r:HS.reference a) = 
+let fresh_sref (#a:Type0) h0 h1 (r:HS.reference a) =
   ~(h0 `HS.contains` r) /\
   HS.frameOf r == HS.(h1.tip) /\
   h1 `HS.contains` r
 
-val accumulate: 
+val accumulate:
   #i:MAC.id -> st:CMA.state i ->
   aadlen:aadlen_32 -> aad:lbuffer (v aadlen) ->
-  txtlen:txtlen_32 -> cipher:lbuffer (v txtlen) -> 
+  txtlen:txtlen_32 -> cipher:lbuffer (v txtlen) ->
   StackInline (CMA.accBuffer i)   // StackInline required for stack-allocated accumulator
-  (requires (fun h0 -> 
-    CMA.(MAC.norm_r h0 st.r) /\
-    Buffer.live h0 aad /\ 
-    Buffer.live h0 cipher /\ 
-    Buffer.disjoint_2 CMA.(MAC.as_buffer st.r) aad cipher))
-  (ensures (fun h0 a h1 -> 
+  (requires (fun h0 ->
+     CMA.(MAC.norm_r h0 st.r) /\
+     Buffer.live h0 aad /\
+     Buffer.live h0 cipher /\
+     Buffer.disjoint_2 CMA.(MAC.as_buffer st.r) aad cipher))
+  (ensures (fun h0 a h1 ->
+    let buf = CMA.abuf a in
     Buffer.modifies_0 h0 h1 /\ // modifies only fresh buffers on the current stack
-    // fresh_sref h0 h1 (Buffer.content (MAC.as_buffer (CMA.abuf a))) /\
-    ~ (h0 `Buffer.contains` (MAC.as_buffer (CMA.abuf a))) /\
-    Buffer.frameOf (MAC.as_buffer (CMA.abuf a)) == h1.tip /\
+    // This doesn't seem to work, so inlining it below:
+    // fresh_sref h0 h1 (Buffer.content (MAC.as_buffer buf)) /\
+    ~(h0 `Buffer.contains` (MAC.as_buffer buf)) /\
+    Buffer.frameOf (MAC.as_buffer buf) == h1.tip /\
+    h1 `Buffer.contains` (MAC.as_buffer buf) /\
     Buffer.live h1 aad /\
     Buffer.live h1 cipher /\
     CMA.acc_inv st a h1 /\
-    (if mac_log then
-       let log = CMA.alog a in
-       fresh_sref h0 h1 log /\
-       //16-12-15 settle for a weaker property? modifies_nothing h0 h1 /\
-       HS.sel h1 log ==
-       encode_both (fst i) aadlen (Buffer.as_seq h1 aad) txtlen (Buffer.as_seq h1 cipher)
-     else
-       Buffer.modifies_0 h0 h1)))
+    (mac_log ==>
+       fresh_sref h0 h1 (CMA.alog a) /\
+       HS.sel h1 (CMA.alog a) ==
+       encode_both (fst i) aadlen (Buffer.as_seq h1 aad) txtlen (Buffer.as_seq h1 cipher)) ))
 
-// TODO FIXME
-#reset-options "--initial_fuel 0 --max_fuel 0 --initial_ifuel 0 --max_ifuel 0 --z3rlimit 200"
-let accumulate #i st aadlen aad txtlen cipher  =
-  let h = ST.get() in 
+
+val frame_modifies_buf_and_ref: #a:Type -> #b:Type -> #c:Type -> h0:mem -> h1:mem ->
+  buf:Buffer.buffer a ->
+  ref:reference b{Buffer.frameOf buf == ref.id} ->
+  buf':Buffer.buffer c -> Lemma 
+  (requires (CMA.modifies_buf_and_ref #a #b buf ref h0 h1 /\
+             (Buffer.frameOf buf' <> Buffer.frameOf buf \/
+              Buffer.disjoint_ref_1 buf' (HS.as_aref ref)) /\
+             Buffer.live h0 buf'))
+  (ensures  (Buffer.live h1 buf'))
+let frame_modifies_buf_and_ref #a #b #c h0 h1 buf ref buf' = ()
+
+
+#reset-options "--max_fuel 0 --max_ifuel 0 --z3rlimit 100"
+let accumulate #i st aadlen aad txtlen cipher =
+  let h = ST.get() in
   let acc = CMA.start st in
   let h0 = ST.get() in
-  assert (mac_log ==> fresh_sref h h0 (CMA.alog acc));
-  Buffer.lemma_reveal_modifies_0 h h0;
-  assert (Buffer.disjoint_2 (MAC.as_buffer (CMA.(abuf acc))) aad cipher);
+  assert (mac_log ==> Buffer.live h0 cipher);
   add_bytes st acc aadlen aad;
-  let h1 = ST.get() in 
+  let h1 = ST.get() in
+  if mac_log then
+    frame_modifies_buf_and_ref h0 h1 CMA.(MAC.as_buffer (CMA.abuf acc)) (CMA.alog acc) cipher;
   add_bytes st acc txtlen cipher;
-  let h2 = ST.get() in 
-  let final_word = Buffer.create 0uy 16ul in 
+  let h2 = ST.get() in  
+  FStar.UInt.pow2_values 32;
+  assert_norm (16 <= pow2 32 - 1);
+  let final_word = Buffer.create 0uy 16ul in
   let h3 = ST.get() in
-  Buffer.lemma_reveal_modifies_0 h2 h3;
-  assert(mac_log ==> h3 `contains` (CMA.alog acc));
+  //Buffer.lemma_reveal_modifies_0 h2 h3;
   let id, _ = i in  // JP: removed a call to Prims.fst
   (match macAlg_of_id id with
     | POLY1305 -> store_lengths_poly1305 aadlen txtlen final_word
     | GHASH    -> store_lengths_ghash    aadlen txtlen final_word);
-  let h4 = ST.get() in 
+  let h4 = ST.get() in
   Buffer.lemma_reveal_modifies_1 final_word h3 h4;
   CMA.frame_acc_inv st acc h2 h3;
   CMA.frame_acc_inv st acc h3 h4;
   CMA.update st acc final_word;
   let h5 = ST.get() in
-  if mac_log then 
+  if mac_log then
     begin
-      let open FStar.Seq in 
+      let open FStar.Seq in
       let al = CMA.alog acc in
-      assert (fresh_sref h h5 al);
-      let cbytes = Buffer.as_seq h cipher in 
-      let abytes = Buffer.as_seq h aad in 
-      let lbytes = Buffer.as_seq h4 final_word in 
-      assert(equal (HS.sel h0 al) createEmpty);
-      Seq.append_empty_r (encode_bytes abytes);
-      assert(equal (HS.sel h1 al) (encode_bytes abytes));
-      assert(equal (HS.sel h2 al) (encode_bytes cbytes @| encode_bytes abytes));
-      assert(equal (HS.sel h5 al) (Seq.cons lbytes (encode_bytes cbytes @| encode_bytes abytes)));
-      assert(equal (HS.sel h5 al) (encode_both (fst i) aadlen abytes txtlen cbytes));
+      let cbytes = Buffer.as_seq h cipher in
+      let abytes = Buffer.as_seq h aad in
+      let lbytes = Buffer.as_seq h4 final_word in
+      append_empty_r (encode_bytes abytes);
+      assert (equal (HS.sel h0 al) createEmpty);
+      assert (equal (HS.sel h1 al) (encode_bytes abytes));
+      assert (equal (HS.sel h2 al) (encode_bytes cbytes @| encode_bytes abytes));
+      assert (equal (HS.sel h5 al) (cons lbytes (encode_bytes cbytes @| encode_bytes abytes)));
+      assert (equal (HS.sel h5 al) (encode_both (fst i) aadlen abytes txtlen cbytes));
       assert(HS.modifies_one h.tip h h0);
       assert(HS.modifies_one h.tip h0 h2);
       assert(HS.modifies_one h.tip h2 h3);
       assert(HS.modifies_one h.tip h3 h4);
       assert(HS.modifies_one h.tip h4 h5);
-      assert(HS.modifies_one h.tip h h5);
-      assert(Buffer.modifies_buf_0 h.tip h h5);
-      Buffer.lemma_intro_modifies_0 h h5
+      assert(HS.modifies_one h.tip h h5)
     end
-  else 
+  else
     begin
-      Buffer.lemma_reveal_modifies_1 (MAC.as_buffer (CMA.(abuf acc))) h0 h2;
+      Buffer.lemma_reveal_modifies_1 (MAC.as_buffer (CMA.abuf acc)) h0 h2;
       Buffer.lemma_reveal_modifies_1 (MAC.as_buffer (CMA.abuf acc)) h4 h5
     end;
+  Buffer.lemma_intro_modifies_0 h h5;
   acc
